$\displaystyle\frac{|\lambda E_n-AB|}{|\lambda E_m-BA|}=\frac{\lambda^n}{\lambda^m}$, 这里 $A_{n\times m}$, $B_{m\times n}$. 

> **证明.** 考虑分块矩阵 $$C=\begin{pmatrix}
\lambda E_n & A\\
B & E_m
\end{pmatrix},$$ 作初等行变换, 有 $$\begin{pmatrix}\lambda E_n & A\\
B & E_m
\end{pmatrix}\sim \begin{pmatrix}\lambda E_n - AB & 0\\
B & E_m
\end{pmatrix},$$ 故 $|C|=|\lambda E_n - AB|$. 另一方面, 作初等列变换, 有 $$\begin{pmatrix}\lambda E_n & A\\
B & E_m
\end{pmatrix}\sim \begin{pmatrix}\lambda E_n & 0\\
B & E_m - \frac{1}{\lambda}BA
\end{pmatrix},$$ 故 $\displaystyle|C|=\lambda^n\cdot\frac{1}{\lambda^m}|\lambda E_m - BA|$. 综上所述, 有 $$|\lambda E_n - AB|=\lambda^{n-m}|\lambda E_m - BA|,$$ 即所需结论.